ModularEngine/src/LogicEngine.FStar/net.fst
@@ -1,36 +1,87 @@
 module Net
 open Types
 open Crypto
+open Authenticate
+open Marshall
 
 type Received :: 'a::* => 'a => E
 assume forall (x:'a) (l:list 'a). In x l && Received l => Received x
 assume forall (s:string). Received (UnicodeStringToBytes s) => Received s
-val methods: Ref (list (principal * (bool -> bytes) * (bytes -> bool)))
-let methods = newref []
-val subscribe: list (principal * (bool -> bytes) * (bytes -> bool)) -> unit
-let subscribe l = (methods:= l)
+assume forall (p:polyterm). (Received (ReprPoly p) => Received p)
 
-val findMethod: principal -> list (principal * (bool -> bytes) * (bytes -> bool)) 
-    -> ((bool->bytes) * (bytes->bool))
-let rec findMethod p l = match l with
-  | [] -> raise (strcat "cannot find methods for " p)
-  | (p', recv, send_to) :: rest ->
-    if p = p' then (recv, send_to)
-    else findMethod p rest
-  
 val receive: unit -> b:bytes{Received b}
 let receive () =
-  match findMethod (Crypto.me) (!methods) with
-    | (recv, _ ) ->
-        let b = recv true in
-      (assume (Received b); b)
-    | _ -> raise "Net.receive"
+  let b = myReceive () true in
+  (assume (Received b); b)
   
 val send: principal -> bytes -> unit
-let send p b =
-  match findMethod p (!methods) with
-    | (_, send_to) ->
-      let _ = send_to b in
-      ()
-    | _ -> raise "Net.send"
+let send p b = 
+  let portNum = lookup_portNum p in
+  let _ = mySend portNum b in ()
+
+type message :: _ =  fun ('P::principal => principal => polyterm => E) => 
+    ((pfrom:principal *
+        pto:principal *
+          i:polyterm{'P pfrom pto i}))
+
+type trivial :: _ = (fun (p:principal) (q:principal) (i:polyterm) => True)
+type jmessage = message (fun (p:principal) (q:principal) (i:polyterm) => (Says p i)) 
+type msg = 
+  | Forwarded : message trivial -> msg
+  | Justified : jmessage -> msg
+
+val polyterm2bytes: i:polyterm -> b:bytes{Serialized i b}
+let polyterm2bytes i =
+  let str = printInfon i in
+    FromUnicodeString str
+
+val msg2bytes: msg -> bytes
+let msg2bytes m =
+  let (me, pkey, skey) = lookup_my_credentials() in
+    match m with
+      | Forwarded ((p,q,i)) -> polyterm2bytes i
+
+      | Justified((p, q, i)) when p=me ->
+          assert (Says me i);
+          let b = polyterm2bytes i in
+          let dsig = rsa_sign me skey i b in
+          let ji = JustifiedPoly (Const (PrincipalConstant p)) i (Const (Bytes dsig)) in 
+            polyterm2bytes ji
+
+val checkMono : i:term -> b:bool{b=true => CheckedInfonMono i}
+let rec checkMono i = match i with 
+  | Var x -> true
+  | Const c -> true
+  | SubstrateQueryTerm _ -> true
+  | App f tms -> 
+      if f=JustifiedInfon then 
+        match tms with 
+          | [(Const (PrincipalConstant p)); i; (Const (Bytes ds))] -> 
+              let pubk = lookup_pubkey p in
+              let bi = polyterm2bytes (MonoTerm i) in 
+              (rsa_verify p pubk (MonoTerm i) bi ds) && checkMono i
+          | _ -> false
+      else for_all<term, CheckedInfonMono> checkMono tms 
+        
+val checkInfon : p:polyterm -> b:bool{b=true => CheckedInfon p}
+let rec checkInfon p = match p with
+  | MonoTerm i -> checkMono i
+  | ForallT xs i -> checkMono i
+  | JustifiedPoly (Const (PrincipalConstant p)) i (Const (Bytes ds)) -> 
+      let pubk = lookup_pubkey p in
+      let bi = polyterm2bytes i in 
+      (rsa_verify p pubk i bi ds) && checkInfon i
+  | _ -> false
+
+val bytes2infon: b:bytes -> option (i:infon{(Received b => Received i)})
+let bytes2infon b = 
+  let s = ToUnicodeString b in 
+    assert (Received b => Received s); 
+    match parseInfon s with 
+      | Some poly when checkInfon poly -> 
+          assert ((ReprPoly poly)=s);
+          assert (Received s => Received poly);
+            Some poly
+      | _ -> None
+    
 
