ModularEngine/src/LogicEngine.FStar/clinical_trials.fst
@@ -194,26 +194,6 @@ let keyMgrPolicy =
       mkRule vars conds actions in
 
   [rule1; rule2]
-     
-(* ---------------- for communication ------------------ *)
-let _ = 
-  let portNum_org = 9200 in
-  let portNum_site = 9201 in
-  let portNum_phys = 9202 in
-  let portNum_keyMgr = 9203 in
-  let org = "org1" in
-  let site = "site1" in
-  let phys =  "phys1" in
-  let keyMgr = "keyMgr" in
-  let org_recv, send_to_org = createComm portNum_org in
-  let site_recv, send_to_site = createComm portNum_site in
-  let phys_recv, send_to_phys = createComm portNum_phys in
-  let keyMgr_recv, send_to_keyMgr = createComm portNum_keyMgr in
-  (subscribe [(org, org_recv, send_to_org);
-              (site, site_recv, send_to_site);
-              (phys, phys_recv, send_to_phys);
-              (keyMgr, keyMgr_recv, send_to_keyMgr)];
-  Keys.addKey org;
-  Keys.addKey site;
-  Keys.addKey phys;
-  Keys.addKey keyMgr)
+
+
+)
